refactoring up to inversion lemma

state/TargetLangIFC.fst
@@ -7,38 +7,61 @@ open FStar.Tactics.Typeclasses
 open Monotonic.IFC.Heap
 open IFC.Heap.ST
 
-(** target_lang is a shallow embedding of STLC **)
-class target_lang (t:Type) = {
+(** witnessable is a shallow embedding of STLC **)
+class witnessable (t:Type) = {
+  // map : t -> lheap -> (#a:Type -> ref a -> Type0) -> Type0; maybe this can be generalized
   shallowly_contained : t -> lheap -> Type0;
   shallowly_low : t -> lheap -> Type0;
 
-  shallowly_witness : x:t -> ST (recall:(unit -> ST unit (fun _ -> True) (fun h0 _ h1 -> h0 == h1 /\ shallowly_contained x h1 /\ shallowly_low x h1)))
+  witness : x:t -> ST (recall:(unit -> ST unit (fun _ -> True) (fun h0 _ h1 -> h0 == h1 /\ shallowly_contained x h1 /\ shallowly_low x h1)))
     (requires (fun h0 -> shallowly_contained x h0 /\ shallowly_low x h0))
     (ensures (fun h0 _ h1 -> h0 == h1))
 }
 
-instance target_lang_unit : target_lang unit = {
-  shallowly_contained = (fun _ _ -> True);
-  shallowly_low = (fun _ _ -> True);
-  shallowly_witness = (fun _ -> (fun () -> ()));
+instance witnessable_ref (t:Type) {| c:witnessable t |} : witnessable (ref t) = {
+  shallowly_contained = (fun (x:ref t) h -> 
+    is_mm x == false /\ contains_pred x h);
+  shallowly_low = (fun (x:ref t) h -> is_low_pred x h);
+  witness = (fun x -> 
+    gst_witness (contains_pred x);
+    gst_witness (is_low_pred x);
+    (fun () -> 
+      gst_recall (contains_pred x);
+      gst_recall (is_low_pred x)))
 }
 
-instance target_lang_int : target_lang int = {
+instance witnessable_unit : witnessable unit = {
   shallowly_contained = (fun _ _ -> True);
   shallowly_low = (fun _ _ -> True);
-  shallowly_witness = (fun _ -> (fun () -> ()));
+  witness = (fun _ -> (fun () -> ()));
 }
 
-instance target_lang_pair (t1:Type) (t2:Type) {| c1:target_lang t1 |} {| c2:target_lang t2 |} : target_lang (t1 * t2) = {
+instance witnessable_int : witnessable int = {
+  shallowly_contained = (fun _ _ -> True);
+  shallowly_low = (fun _ _ -> True);
+  witness = (fun _ -> (fun () -> ()));
+}
+
+instance witnessable_arrow 
+  (t1:Type) (t2:Type)
+  (pre:t1 -> lheap -> Type0)
+  (post:t1 -> lheap -> t2 -> lheap -> Type0) // TODO: one cannot have pre-post depending on outside things.
+: witnessable (x:t1 -> ST t2 (pre x) (post x)) = {
+  shallowly_contained = (fun _ _ -> True);
+  shallowly_low = (fun _ _ -> True);
+  witness = (fun _ -> (fun () -> ()));
+}
+
+instance witnessable_pair (t1:Type) (t2:Type) {| c1:witnessable t1 |} {| c2:witnessable t2 |} : witnessable (t1 * t2) = {
   shallowly_contained = (fun (x1, x2) h -> c1.shallowly_contained x1 h /\ c2.shallowly_contained x2 h);
   shallowly_low = (fun (x1, x2) h -> c1.shallowly_low x1 h /\ c2.shallowly_low x2 h);
-  shallowly_witness = (fun (x1,x2) -> 
-    let w1 = c1.shallowly_witness x1 in
-    let w2 = c2.shallowly_witness x2 in
+  witness = (fun (x1, x2) -> 
+    let w1 = c1.witness x1 in
+    let w2 = c2.witness x2 in
     (fun () -> w1 (); w2 ()))
 }
 
-instance target_lang_sum (t1:Type) (t2:Type) {| c1:target_lang t1 |} {| c2:target_lang t2 |} : target_lang (either t1 t2) = {
+instance witnessable_sum (t1:Type) (t2:Type) {| c1:witnessable t1 |} {| c2:witnessable t2 |} : witnessable (either t1 t2) = {
   shallowly_contained = (fun x h ->
     match x with
     | Inl x1 -> c1.shallowly_contained x1 h
@@ -47,48 +70,108 @@ instance target_lang_sum (t1:Type) (t2:Type) {| c1:target_lang t1 |} {| c2:targe
     match x with
     | Inl x1 -> c1.shallowly_low x1 h
     | Inr x2 -> c2.shallowly_low x2 h);
-  shallowly_witness = (fun x -> 
+  witness = (fun x -> 
     match x with 
-    | Inl x1 -> (let w = c1.shallowly_witness x1 in (fun () -> w ()))
-    | Inr x2 -> (let w = c2.shallowly_witness x2 in (fun () -> w ())))
+    | Inl x1 -> (let w = c1.witness x1 in (fun () -> w ()))
+    | Inr x2 -> (let w = c2.witness x2 in (fun () -> w ())))
 }
 
-instance target_lang_ref (t:Type) {| c:target_lang t |} : target_lang (ref t) = {
-  shallowly_contained = (fun (x:ref t) h -> 
-    is_mm x == false /\ contains_pred x h);
-  shallowly_low = (fun (x:ref t) h -> is_low_pred x h);
-  shallowly_witness = (fun x -> 
-    gst_witness (contains_pred x);
-    gst_witness (is_low_pred x);
-    (fun () -> 
-      gst_recall (contains_pred x);
-      gst_recall (is_low_pred x)))
-}
+(** *** Elaboration of types to F* *)
 
-open FStar.Preorder
+unfold let shallowly_contained_low (#a:Type) {| c:witnessable a |} (v:a) (h:lheap) =
+  c.shallowly_contained v h /\ c.shallowly_low v h
+
+unfold let pre_tgt_arrow
+  (#t1:Type) {| c1 : witnessable t1 |}
+  (#inv:lheap -> Type0)
+  (x:t1) (h0:lheap) =
+  inv h0 /\
+  shallowly_contained_low #t1 #c1 x h0
+
+unfold let post_tgt_arrow
+  (#t1:Type) {| c1 : witnessable t1 |}
+  (#t2:Type) {| c2 : witnessable t2 |}
+  (#inv:lheap -> Type0)
+  (x:t1) (h0:lheap) (r:t2) (h1:lheap) =
+  inv h1 /\
+  modifies_only_label Low h0 h1 /\                       (* allows low references to be modified *)
+  modifies_classification Set.empty h0 h1 /\             (* no modifications of the classification *)
+  shallowly_contained_low #t2 #c2 r h1
+
+let mk_tgt_arrow 
+  (inv:lheap -> Type0)
+  (t1:Type) {| c1 : witnessable t1 |}
+  (t2:Type) {| c2 : witnessable t2 |}
+= x:t1 -> ST t2 
+    (requires (pre_tgt_arrow #t1 #c1 #inv x ))
+    (ensures (post_tgt_arrow #t1 #c1 #t2 #c2 #inv x))
+
+open STLC
+
+let rec _elab_typ (t:typ) (inv:lheap -> Type0): tt:Type0 & witnessable tt =
+  match t with
+  | TArr t1 t2 -> begin
+    let tt1 = _elab_typ t1 inv in
+    let tt2 = _elab_typ t2 inv in
+    (| mk_tgt_arrow inv (dfst tt1) #(dsnd tt1) (dfst tt2) #(dsnd tt2),
+       witnessable_arrow (dfst tt1) (dfst tt2) pre_tgt_arrow post_tgt_arrow
+    |)
+  end 
+  | TUnit -> (| unit, witnessable_unit |)
+  | TNat -> (| int, witnessable_int |)
+  | TSum t1 t2 ->
+    let (| tt1, c_tt1 |) = _elab_typ t1 inv in
+    let (| tt2, c_tt2 |) = _elab_typ t2 inv in
+    (| either tt1 tt2, witnessable_sum tt1 tt2 #c_tt1 #c_tt2 |)
+  | TPair t1 t2 ->
+    let (| tt1, c_tt1 |) = _elab_typ t1 inv in
+    let (| tt2, c_tt2 |) = _elab_typ t2 inv in
+    (| (tt1 * tt2), witnessable_pair tt1 tt2 #c_tt1 #c_tt2 |)
+  | TRef t ->
+    let (| tt, c_tt |) = _elab_typ t inv in
+    (| ref tt, witnessable_ref tt #c_tt |)
 
 let inv_contains_points_to_contains (h:lheap) =
-  (* TODO: the forall on target_lang is creating problems in proofs. 
-    One solution would be to quantify over STLC types and use elab_typ. However,
-    the definitions depend one on other.
-  *)
-  (forall (a:Type) (c:target_lang a) (r:ref a).
-    shallowly_contained r h ==> c.shallowly_contained (sel h r) h)
-
-  (* (forall (tt:base_target_type). forall (r:ref (el tt)). *)
-  (*   shallowly_contained r h ==> f_shallowly_contained tt (sel h r) h) *)
+  (forall (a:typ) (inv:lheap -> Type0).
+    let tt = _elab_typ a inv in
+    forall (r:ref (dfst tt)).
+      (witnessable_ref (dfst tt) #(dsnd tt)).shallowly_contained r h ==> 
+        (dsnd tt).shallowly_contained (sel h r) h)
 
 let inv_low_points_to_low (h:lheap) =
-  (forall (a:Type) (c:target_lang a) (r:ref a).
-    shallowly_low r h ==> c.shallowly_low (sel h r) h)
+  (forall (a:typ) (inv:lheap -> Type0).
+    let tt = _elab_typ a inv in
+    forall (r:ref (dfst tt)).
+      (witnessable_ref (dfst tt) #(dsnd tt)).shallowly_low r h ==> 
+        (dsnd tt).shallowly_low (sel h r) h)
 
 let inv_low_contains (h:lheap) = 
   inv_contains_points_to_contains h /\
   inv_low_points_to_low h
 
-unfold let shallowly_contained_low (#a:Type) {| c:target_lang a |} (v:a) (h:lheap) =
-  c.shallowly_contained v h /\ c.shallowly_low v h
+let elab_typ (t:typ) : Type =
+  dfst (_elab_typ t inv_low_contains)
 
+let elab_typ_tgt (t:typ) : witnessable (elab_typ t)=
+  dsnd (_elab_typ t inv_low_contains)
+
+let eliminate_inv_low (h:lheap) (a:typ) (r:ref (elab_typ a)) :
+  Lemma
+    (requires (inv_low_points_to_low h))
+    (ensures (
+        (witnessable_ref (elab_typ a) #(elab_typ_tgt a)).shallowly_low r h ==> 
+          (elab_typ_tgt a).shallowly_low (sel h r) h
+    )) = ()
+
+let eliminate_inv_contains (h:lheap) (a:typ) (r:ref (elab_typ a)) :
+  Lemma
+    (requires (inv_contains_points_to_contains h))
+    (ensures (
+        (witnessable_ref (elab_typ a) #(elab_typ_tgt a)).shallowly_contained r h ==> 
+          (elab_typ_tgt a).shallowly_contained (sel h r) h
+    )) = ()
+
+(** ** Examples **) 
 effect IST (a:Type) (pre:st_pre) (post: (h:lheap -> Tot (st_post' a (pre h)))) =
   ST a 
     (requires (fun h0 -> 
@@ -98,76 +181,7 @@ effect IST (a:Type) (pre:st_pre) (post: (h:lheap -> Tot (st_post' a (pre h)))) =
       inv_low_contains h1 /\
       post h0 r h1))
 
-unfold let pre_tgt_arrow
-  (#t1:Type) (x:t1) {| tgtx:target_lang t1 |}
-  (h0:lheap) =
-  shallowly_contained_low #t1 #tgtx x h0
-
-unfold let post_tgt_arrow
-  (#t1:Type) (x:t1) {| tgtx:target_lang t1 |}
-  (#t2:Type) {| tgtr : target_lang t2 |}
-  (h0:lheap) (r:t2) (h1:lheap) =
-  modifies_only_label Low h0 h1 /\                                       (* allows low references to be modified *)
-  modifies_classification Set.empty h0 h1 /\                             (* no modifications of the classification *)
-  shallowly_contained_low r h1
-
-let mk_tgt_arrow 
-  (t1:Type)
-  {| tgt_t1: target_lang t1 |}
-  (t2:Type)
-  {| c2 : target_lang t2 |}
-= x:t1 -> IST t2 
-    (requires (pre_tgt_arrow x #tgt_t1))
-    (ensures (post_tgt_arrow x #tgt_t1 #t2 #c2))
-
-instance target_lang_arrow 
-  (t1:Type)
-  {| target_lang t1 |}
-  (t2:Type)
-  {| target_lang t2 |}
-  : target_lang (mk_tgt_arrow t1 t2) = {
-    shallowly_contained = (fun _ _ -> True);
-    shallowly_low = (fun _ _ -> True);
-    shallowly_witness = (fun _ -> (fun () -> ()));
-  }
-
-
-open STLC
-
-(** *** Elaboration of types to F* *)
-let rec _elab_typ (t:typ) : tt:Type0 & target_lang tt =
-  match t with
-  | TArr t1 t2 -> begin
-    let tt1 = _elab_typ t1 in
-    let tt2 = _elab_typ t2 in
-    (| mk_tgt_arrow      (dfst tt1) #(dsnd tt1) (dfst tt2) #(dsnd tt2),
-       target_lang_arrow (dfst tt1) #(dsnd tt1) (dfst tt2) #(dsnd tt2)
-    |)
-  end 
-  | TUnit -> (| unit, target_lang_unit |)
-  | TNat -> (| int, target_lang_int |)
-  | TSum t1 t2 ->
-    let (| tt1, c_tt1 |) = _elab_typ t1 in
-    let (| tt2, c_tt2 |) = _elab_typ t2 in
-    (| either tt1 tt2, target_lang_sum tt1 tt2 #c_tt1 #c_tt2 |)
-  | TPair t1 t2 ->
-    let (| tt1, c_tt1 |) = _elab_typ t1 in
-    let (| tt2, c_tt2 |) = _elab_typ t2 in
-    (| (tt1 * tt2), target_lang_pair tt1 tt2 #c_tt1 #c_tt2 |)
-  | TRef t ->
-    let (| tt, c_tt |) = _elab_typ t in
-    (| ref tt, target_lang_ref tt #c_tt |)
-
-let elab_typ (t:typ) : Type =
-  dfst (_elab_typ t)
-
-let elab_typ_tgt (t:typ) : target_lang (elab_typ t)=
-  dsnd (_elab_typ t)
-
-
-
-(** ** Examples **) 
-let write' (#t:Type) {| c:target_lang t |} (r:ref t) (v:t) 
+let write' (#t:Type) {| c:witnessable t |} (r:ref t) (v:t) 
 : IST unit
   (requires (fun h0 -> 
     shallowly_contained_low r h0 /\
@@ -183,8 +197,8 @@ let write' (#t:Type) {| c:target_lang t |} (r:ref t) (v:t)
   assume (inv_contains_points_to_contains h1);
   ()
 
-let _alloc (#a:Type) (#rel:preorder a) (init:a)
-: IST (mref a rel) (fun h -> True) (alloc_post #a #rel init)
+let _alloc (#a:Type) (init:a)
+: IST (ref a) (fun h -> True) (alloc_post #a init)
 =
   let r = alloc init in
   let h1 = get () in
@@ -192,7 +206,7 @@ let _alloc (#a:Type) (#rel:preorder a) (init:a)
   assume (inv_contains_points_to_contains h1);
   r
 
-let declassify_low' (#a:Type) {| c:target_lang a |} (r:ref a) : ST unit
+let declassify_low' (#a:Type) {| c:witnessable a |} (r:ref a) : ST unit
   (fun h -> shallowly_contained r h /\ inv_contains_points_to_contains h)
   (fun h0 () h1 -> 
     inv_contains_points_to_contains h1 /\
@@ -203,7 +217,7 @@ let declassify_low' (#a:Type) {| c:target_lang a |} (r:ref a) : ST unit
   let h1 = get () in
   assume (inv_contains_points_to_contains h1)
 
-val alloc' (#a:Type) {| c:target_lang a |} (init:a)
+val alloc' (#a:Type) {| c:witnessable a |} (init:a)
 : IST (ref a)
   (requires (fun h0 ->
     shallowly_contained_low init h0))
@@ -233,15 +247,11 @@ val ctx_update_multiple_refs_test :
 let ctx_update_multiple_refs_test (x:ref (ref int)) =
   gst_witness (contains_pred x);
   gst_witness (is_low_pred x);
-  let cb : elab_typ (TArr (TRef TNat) TUnit) = (fun (y:ref int) -> 
+  let cb : elab_typ (TArr (TRef TNat) TUnit) = (fun (y:ref int) ->
     let h0 = get () in
     gst_recall (contains_pred x);
     let ix : ref int = !x in
-    eliminate forall (a:Type) (c:target_lang a) (r:ref a). shallowly_contained r h0 ==>
-      c.shallowly_contained (sel h0 r) h0 with (ref int) (solve) x;
     gst_recall (is_low_pred x);    
-    eliminate forall (a:Type) (c:target_lang a) (r:ref a). shallowly_low r h0 ==>
-      c.shallowly_low (sel h0 r) h0 with (ref int) (solve) x;
     write' ix (!ix + 1);
     let h1 = get () in
     write' x y;
@@ -261,10 +271,8 @@ val ctx_HO_test1 :
 let ctx_HO_test1 (xs:ref ((ref int) * ref int)) =
   let (x', x'') = !xs in
   let h0 = get () in
-  eliminate forall (a:Type) (c:target_lang a) (r:ref a). shallowly_contained r h0 ==>
-    c.shallowly_contained (sel h0 r) h0 with ((ref int) * (ref int)) (solve) xs;
-  eliminate forall (a:Type) (c:target_lang a) (r:ref a). shallowly_low r h0 ==>
-    c.shallowly_low (sel h0 r) h0 with ((ref int) * (ref int)) (solve) xs;
+  eliminate_inv_contains h0 (TPair (TRef TNat) (TRef TNat)) xs;
+  eliminate_inv_low h0 (TPair (TRef TNat) (TRef TNat)) xs;
   write' xs (x', x');
   gst_witness (is_low_pred xs);
   gst_witness (is_low_pred x');
@@ -299,18 +307,17 @@ let ctx_swap_ref_test (x:ref (ref int)) =
   let cb : elab_typ (TArr (TRef (TRef TNat)) TUnit) = (fun (y: ref (ref int)) ->
     let h0 = get () in
     gst_recall (contains_pred x);
-    eliminate forall (a:Type) (c:target_lang a) (r:ref a). shallowly_contained r h0 ==>
-      c.shallowly_contained (sel h0 r) h0 with (ref int) (solve) x;
     gst_recall (is_low_pred x);
-    eliminate forall (a:Type) (c:target_lang a) (r:ref a). shallowly_low r h0 ==>
-      c.shallowly_low (sel h0 r) h0 with (ref int) (solve) x;
-
+    eliminate_inv_contains h0 (TRef TNat) x;
+    eliminate_inv_low h0 (TRef TNat) x;
+    
     let z = !x in
     let t = !y in
     write' x t;
     let h1 = get () in
     write' y z;
     let h2 = get () in
+
     lemma_modifies_only_label_trans Low h0 h1 h2;
     assert (modifies_only_label Low h0 h2); // we have an SMT Pat for this, but it does not kick in
     assert (modifies_classification Set.empty h0 h2);
@@ -363,37 +370,94 @@ val progr_sep_test:
 let progr_sep_test #rp f = (** If this test fails, it means that the spec of f does not give [automatically] separation  **)
   f ()
 
-let lemma (#a:Type) {| c:target_lang a |} (x:a) (h0 h1:lheap) : Lemma (
+let lemma (#a:Type) {| c:witnessable a |} (x:a) (h0 h1:lheap) : Lemma (
   h0 `lheap_rel` h1 /\ shallowly_low x h0 ==> shallowly_low x h1
 ) = admit ()
 
+open FStar.Calc
 
-let lemma123 (r:ref int) (h0 h1:lheap) : Lemma
+(** Nik's workaround:
+Here's a possible workaround until we figure out if and how to support reasoning about disequalities on effectful function types
+Is it possible for you to work with a type isomorphic to (int -> Dv int)? For example:
+type wrap_div (a:Type) = | WrapDiv of a
+let unwrap_div (x:wrap_div 'a) : 'a = match x with | WrapDiv y -> y
+
+let _ = assert (int =!= wrap_div (int -> Dv int))
+I.e., use a fresh inductive type to wrap each effecftul function type? So, you'd have wrap_div, wrap_st etc?
+*)
+let rec inversion (a:typ) (inv:lheap -> Type0) (xa:typ) :
+  Lemma
+    (requires (dfst (_elab_typ a inv) == elab_typ xa))
+    (ensures (a == xa /\ dsnd (_elab_typ a inv) == elab_typ_tgt xa)) =
+    match a, xa with
+    | TNat, TNat -> ()
+    | TUnit, TUnit -> ()
+    | TSum t1 t2, TSum t1' t2' -> begin
+      assume (dfst (_elab_typ t1 inv) == elab_typ t1');
+      inversion t1 inv t1';
+      assume (dfst (_elab_typ t2 inv) == elab_typ t2');
+      inversion t2 inv t2'
+    end
+    | TPair t1 t2, TPair t1' t2' -> begin
+      assume (dfst (_elab_typ t1 inv) == elab_typ t1');
+      inversion t1 inv t1';
+      assume (dfst (_elab_typ t2 inv) == elab_typ t2');
+      inversion t2 inv t2'
+    end
+    | TRef t, TRef t' -> begin
+      assume (dfst (_elab_typ t inv) == elab_typ t');
+      inversion t inv t'
+    end
+    | TArr x y, TArr x' y' ->
+      assume (dfst (_elab_typ x inv) == elab_typ x');
+      inversion x inv x';
+      assume (dfst (_elab_typ y inv) == elab_typ y');
+      inversion y inv y';
+      assume (inv == inv_low_contains)
+    | _, _ -> admit () (* TODO: other cases are impossible because of the pre-condition*)
+
+let lemma_declassify_preserves_inv (xa:typ) (x:ref (elab_typ xa)) (h0 h1:lheap) : Lemma
   (requires (modifies_none h0 h1 /\
             h0 `lheap_rel` h1 /\
             equal_dom h0 h1 /\
-            modifies_classification (only r) h0 h1 /\
-            shallowly_contained r h0 /\ 
-            shallowly_contained_low r h1 /\
+            modifies_classification (only x) h0 h1 /\
+            (elab_typ_tgt (TRef xa)).shallowly_contained x h0 /\ 
+            shallowly_contained_low #(elab_typ xa) #(elab_typ_tgt xa) (sel h0 x) h0 /\
+            shallowly_contained_low #(ref (elab_typ xa)) #(elab_typ_tgt (TRef xa)) x h1 /\
             inv_low_points_to_low h0))
   (ensures (inv_low_points_to_low h1)) = 
-  introduce forall (a:Type) (c:target_lang a) (r:ref a). 
-    shallowly_low r h1 ==> c.shallowly_low (sel h1 r) h1
+  introduce forall (a:typ) (inv:lheap -> Type0).
+    let tt = _elab_typ a inv in
+    forall (r:ref (dfst tt)).
+      (witnessable_ref (dfst tt) #(dsnd tt)).shallowly_low r h1 ==> 
+        (dsnd tt).shallowly_low (sel h1 r) h1
   with begin
-    introduce shallowly_low r h1
-      ==> c.shallowly_low (sel h1 r) h1
-    with _. begin
-      introduce shallowly_low r h0 ==> c.shallowly_low (sel h1 r) h1 
-      with _. lemma (sel h0 r) h0 h1;
-      
-      introduce ~(shallowly_low r h0) ==> c.shallowly_low (sel h1 r) h1
+    let tt = _elab_typ a inv in
+    let refw = witnessable_ref (dfst tt) #(dsnd tt) in
+    introduce forall (r:ref (dfst tt)).
+      refw.shallowly_low r h1 ==> 
+        (dsnd tt).shallowly_low (sel h1 r) h1
+    with begin
+      introduce refw.shallowly_low r h1 ==> 
+          (dsnd tt).shallowly_low (sel h1 r) h1
       with _. begin
-        assert (shallowly_low r h1);
-        let v : int = sel h1 r in 
-        let c' : target_lang int = solve in
-        assert (c'.shallowly_low v h1);
-        assume (c.shallowly_low v h1); (* TODO: idk how to get rid of this *)
-        ()
+        introduce refw.shallowly_low r h0 ==> (dsnd tt).shallowly_low (sel h1 r) h1 
+        with _. lemma #(dfst tt) #(dsnd tt) (sel h0 r) h0 h1;
+        
+        introduce ~(refw.shallowly_low r h0) ==> (dsnd tt).shallowly_low (sel h1 r) h1
+        with _. begin
+          assert (addr_of r == addr_of x);
+          lemma_sel_same_addr' h1 x r;
+          assert (dfst tt == elab_typ xa);
+          inversion a inv xa;
+          assert (dsnd tt == elab_typ_tgt xa);
+
+          assert ((elab_typ_tgt xa).shallowly_low (sel h0 x) h0);
+          lemma #(elab_typ xa) #(elab_typ_tgt xa) (sel h0 x) h0 h1;
+          assert (sel h0 x == sel h1 x);
+          assert ((elab_typ_tgt xa).shallowly_low (sel h1 x) h1);
+          assert ((dsnd tt).shallowly_low (sel h1 r) h1)
+        end
       end
     end
   end
@@ -407,9 +471,10 @@ val progr_sep_test_alloc:
       label_of rp h0 == High))
     (ensures (fun h0 _ h1 -> True))
 let progr_sep_test_alloc rp f =
+  let h0 = get () in
   declassify_low' rp;
   let h1 = get () in
-  assume (inv_low_points_to_low h1);
+  lemma_declassify_preserves_inv TNat rp h0 h1;
   let r = f rp in  
   r
 
@@ -422,12 +487,16 @@ val progr_sep_test_nested:
       label_of rp h0 == High))
     (ensures (fun h0 _ h1 -> True))
 let progr_sep_test_nested rp f =
+  let h0 = get () in
+  eliminate_inv_contains h0 (TRef TNat) rp;
+
   let p : ref int = !rp in
-  declassify_low' rp;
   declassify_low' p;
   let h1 = get () in
-  assume (inv_low_points_to_low h1);
-
+  lemma_declassify_preserves_inv TNat p h0 h1;
+  declassify_low' rp;
+  let h2 = get () in
+  lemma_declassify_preserves_inv (TRef TNat) rp h1 h2;
   // let r = alloc' (!rp) in (* <-- needed a copy here! *) 
   f rp
 
@@ -464,15 +533,16 @@ val progr_passing_callback_test:
 // TODO: the callback of the program should be able to modify rp
 let progr_passing_callback_test rp rs f =
   let secret: ref int = _alloc 0 in
+  let h0 = get () in
   declassify_low' secret;
+  let h1 = get () in
+  lemma_declassify_preserves_inv TNat secret h0 h1;
   gst_witness (contains_pred secret);
   gst_witness (is_low_pred secret);
   let cb: elab_typ (TArr TUnit TUnit) = (fun () -> 
     gst_recall (contains_pred secret);
     gst_recall (is_low_pred secret);
     write' secret (!secret + 1)) in
-  let h1 = get () in
-  assume (inv_low_points_to_low h1);
   f cb;
   ()
 
@@ -501,9 +571,9 @@ val elab_apply_arrow :
   t1:typ ->
   t2:typ ->
   f:elab_typ (TArr t1 t2) ->
-  (let tt1 = _elab_typ t1 in
-   let tt2 = _elab_typ t2 in
-   mk_tgt_arrow (dfst tt1) #(dsnd tt1) (dfst tt2) #(dsnd tt2))
+  (let tt1 = _elab_typ t1 inv_low_contains in
+   let tt2 = _elab_typ t2 inv_low_contains in
+   mk_tgt_arrow inv_low_contains (dfst tt1) #(dsnd tt1) (dfst tt2) #(dsnd tt2))
 let elab_apply_arrow t1 t2 f x = f x
 
 let cast_TArr #t1 #t2 (f : elab_typ (TArr t1 t2)) (t:typ) (#_:squash (t == TArr t1 t2)) : elab_typ t = f
@@ -520,7 +590,7 @@ let vextend #t (x:elab_typ t) (#g:context) (ve:vcontext g) :
   ST (vcontext (extend t g))
     (requires (fun h0 -> shallowly_contained_low #_ #(elab_typ_tgt t) x h0))
     (ensures (fun h0 r h1 -> h0 == h1)) =
-  let w = (elab_typ_tgt t).shallowly_witness x in
+  let w = (elab_typ_tgt t).witness x in
   fun y -> 
     if y = 0 then (w (); x) else ve (y-1)
 
@@ -532,8 +602,8 @@ let rec elab_exp
   (tyj:typing g e t)
   (ve:vcontext g)
   : IST (elab_typ t) 
-     (requires (pre_tgt_arrow () #target_lang_unit))
-     (ensures (post_tgt_arrow () #_ #(elab_typ t) #(elab_typ_tgt t))) =
+     (requires (pre_tgt_arrow #unit #witnessable_unit #inv_low_contains ()))
+     (ensures (post_tgt_arrow #_ #_ #(elab_typ t) #(elab_typ_tgt t) #inv_low_contains ())) =
   let h0 = get () in
   match tyj with
   | TyUnit -> ()
@@ -557,7 +627,7 @@ let rec elab_exp
   end
 
   | TyAbs tx #_ #tres tyj_body ->
-    let w : mk_tgt_arrow (elab_typ tx) #(elab_typ_tgt tx) (elab_typ tres) #(elab_typ_tgt tres) = 
+    let w : mk_tgt_arrow inv_low_contains (elab_typ tx) #(elab_typ_tgt tx) (elab_typ tres) #(elab_typ_tgt tres) = 
       (fun (x:elab_typ tx) -> 
         elab_exp tyj_body (vextend #tx x ve))
     in
@@ -570,7 +640,7 @@ let rec elab_exp
   | TyApp #_ #_ #_ #tx #tres tyj_f tyj_x ->
     assert ((elab_typ t) == (elab_typ tres));
     let x : elab_typ tx = elab_exp tyj_x ve in
-    let wx = (elab_typ_tgt tx).shallowly_witness x in
+    let wx = (elab_typ_tgt tx).witness x in
     let f : elab_typ (TArr tx tres) = elab_exp tyj_f ve in
     wx ();
     elab_apply_arrow tx tres f x
@@ -585,12 +655,12 @@ let rec elab_exp
     let vc : either (elab_typ tl) (elab_typ tr) = elab_exp tyj_c ve in
     match vc with 
     | Inl x -> 
-      let wx = (elab_typ_tgt tl).shallowly_witness x in
+      let wx = (elab_typ_tgt tl).witness x in
       let f : elab_typ (TArr tl tres) = elab_exp tyj_l ve in
       wx ();
       elab_apply_arrow tl tres f x
     | Inr y ->
-      let wy = (elab_typ_tgt tr).shallowly_witness y in
+      let wy = (elab_typ_tgt tr).witness y in
       let f : elab_typ (TArr tr tres) = elab_exp tyj_r ve in
       wy ();
       elab_apply_arrow tr tres f y
@@ -604,7 +674,7 @@ let rec elab_exp
     snd #(elab_typ tf) #(elab_typ ts) v
   | TyPair #_ #_ #_ #tf #ts tyj_f tyj_s->
     let vf : elab_typ tf = elab_exp tyj_f ve in
-    let wvf = (elab_typ_tgt tf).shallowly_witness vf in
+    let wvf = (elab_typ_tgt tf).witness vf in
     let vs : elab_typ ts = elab_exp tyj_s ve in
     wvf ();
     (vf, vs)
